pbt/fpc-pair.sig
@@ -1,5 +1,5 @@
 sig fpc-pair.
-accum_sig kernel.
+accum_sig dep-kernel.
 
 % Certificate pairing
 type   pair   cert -> cert -> cert.
