examples/list_queries.v
@@ -2,75 +2,8 @@ From elpi Require Import elpi.
 Require Import Arith. 
 Require Import Coq.Lists.List.
 Import ListNotations.
-Require Import pbt.
 Require Import dep_pbt.
 Load list.
-
-(* ****** QUERIES****** *)
-
-(*original query*)
-Goal forall xs rs,
-is_natlist xs ->
-ordered_bad xs -> insert 0 xs rs ->
-ordered_bad rs.
-intros xs rs Gen H1 H2.
-elpi pbt (Gen /\ H1) (H2) 5 (rs). (* why rs?*) 
-
-elpi pbt (Gen /\ H1) (H2) 5 (xs /\ rs).
-Abort.
-
-(* with generation only of natlist*)
-
-Goal forall xs rs,
-is_natlist xs -> ordered_bad xs -> insert 0 xs rs -> ordered_bad rs.
-intros xs rs Gen H1 H2.
-elpi pbt (Gen) (H1 /\ H2) 5 (rs). 
-Abort.
-
-(* generating both nat and natlist*)
-
-Goal forall x xs rs,
-
-is_nat x -> is_natlist xs -> ordered_bad xs -> insert x xs rs -> ordered_bad rs.
-
-intros x xs rs GenN GenL  H1 H2.
-elpi pbt (GenN /\ GenL ) (H1 /\ H2) 5 (rs). 
-Abort.
-
-(* This property is true *)
-Goal forall xs rs, is_natlist xs -> rev xs rs -> rev rs xs.
-intros xs rs Gen H.
-Fail elpi pbt (Gen) (H) 5 (xs).
-Abort.
-
-(* This property is false *)
-Goal forall xs rs, is_natlist xs -> rev xs rs -> xs = rs.
-intros xs rs Gen H.
-elpi pbt (Gen) (H) 4 (rs).
-Abort.
-
-(* true *)
-Goal forall xs rs, is_natlist xs -> rev xs rs -> rev2 xs rs.
-intros xs rs Gen HR.
-Fail elpi pbt (Gen) (HR) 5 (xs).
-Abort.
-
-(* false *)
-Goal forall xs ys aps raps rxs rys,
-is_natlist xs -> is_natlist ys -> 
-append xs ys aps -> rev xs rxs -> rev ys rys ->
-rev aps raps -> append rxs rys raps.
-intros.
-elpi pbt (H /\ H0) (H1 /\ H2 /\ H3 /\ H4) 4 (xs /\ ys).
-Abort.
-
-Goal forall x x' y: list nat,
-is_natlist x -> 
-append [0] x x' -> rev x y -> rev y x'.
-intros.
-elpi pbt (H) (H0 /\ H1) 5 (x).
-Abort.
-
 
 (* ****** DEP QUERIES****** *)
 
@@ -94,13 +27,13 @@ Abort.
 (* This property is true *)
 Goal forall (xs rs : list nat), rev xs rs -> rev rs xs.
 intros xs rs  H.
-Fail elpi dep_pbt 5 (H) (xs).
+Fail elpi dep_pbt 3 (H) (xs).
 Abort.
 
 (* true *)
 Goal forall (xs rs : list nat), rev xs rs -> rev2 xs rs.
 intros xs rs HR.
-Fail elpi dep_pbt 5 (HR) (xs).
+Fail elpi dep_pbt 2 (HR) (xs).
 Abort.
 
 (* false *)
@@ -117,8 +50,8 @@ intros.
 elpi dep_pbt 3 (H /\ H0) (x).
 Abort.
 
-Goal forall x y: list nat,
+(*Goal forall x y: list nat,
 rev (app [2] x) y.
 
 intros.
-elpi dep_pbt 3 (True) (x).
+elpi dep_pbt 3 (True) (x).*)
