examples/toy.v
@@ -1,5 +1,9 @@
-(* A toy examples to mix comuptation and deduction *)
+(* A toy examples to mix comptation and deduction *)
+From elpi Require Import elpi.
+ Require Import Arith List. Import ListNotations.
 
+ Require Import dep_pbt.
+ Require Import dprolog.
 Inductive tm : Type :=
   | C : nat -> tm         (* Constant *)
   | P : tm -> tm -> tm.   (* Plus *)
@@ -30,3 +34,12 @@ Goal
         (P (C 2) (C 4)).
 Proof.
   apply ST_Plus1. apply ST_PlusConstConst.  Qed.
+
+  Lemma g1:   
+  (P (C 3) (C 0))
+===>
+
+  (C 3).
+  elpi dprolog 5.
+  Qed.
+  Print g1.
